moved Cert_co to a new file

src/simulation/CertExecution2.v
@@ -18,6 +18,8 @@ Require Import ExtTraversalConfig.
 
 Require Import ImmProperties.
 
+Require Import Cert_co.
+
 Set Implicit Arguments.
 Remove Hints plus_n_O.
 
@@ -95,6 +97,7 @@ Notation "'Acq/Rel'" := (fun a => is_true (is_ra Glab a)).
 Notation "'Sc'" := (fun a => is_true (is_sc Glab a)).
 Notation "'xacq'" := (fun a => is_true (is_xacq Glab a)).
 
+
 Variable T : trav_config.
 Variable S : actid -> Prop.
 
@@ -102,6 +105,8 @@ Notation "'I'" := (issued T).
 Notation "'C'" := (covered T).
 
 Variable thread : BinNums.positive.
+
+Notation "'cert_co'" := (cert_co G T thread).
 
 Hypothesis WF : Wf G.
 Hypothesis WF_SC : wf_sc G sc.
@@ -571,186 +576,6 @@ Proof using All.
   apply dom_ppo_D.
 Qed.
 
-(******************************************************************************)
-(**  new co relation  *)
-(******************************************************************************)
-
-Definition cert_co_base := I ∪₁ W_ex G.
-Lemma cert_co_base_alt : cert_co_base ≡₁ I ∪₁ W_ex G ∩₁ Tid_ thread.
-Proof using WF IT_new_co.
-  clear -WF IT_new_co.
-  unfold cert_co_base.
-  split; [|basic_solver].
-  unionL; [basic_solver|].
-  rewrite WF.(W_ex_eq_EW_W_ex) at 1.
-  rewrite <- IT_new_co. basic_solver.
-Qed.
-
-Lemma I_in_cert_co_base : I ⊆₁ cert_co_base.
-Proof using. unfold cert_co_base. basic_solver. Qed.
-Lemma IST_in_cert_co_base : I ∪₁ S ∩₁ Tid_ thread ⊆₁ cert_co_base.
-Proof using S_I_in_W_ex.
-  rewrite AuxRel.set_subset_union_minus with (s:=S ∩₁ Tid_ thread) (s':=I).
-  rewrite S_I_in_W_ex.
-  unfold cert_co_base. clear. basic_solver.
-Qed.
-
-Definition cert_co := new_co G cert_co_base (E ∩₁ W ∩₁ Tid_ thread).
-
-Lemma IST_new_co : cert_co_base ∪₁ E ∩₁ W ∩₁ Tid_ thread ≡₁ E ∩₁ W.
-Proof using WF S_in_W ST_in_E IT_new_co.
-  rewrite <- IT_new_co at 2.
-  rewrite cert_co_base_alt.
-  rewrite WF.(W_ex_eq_EW_W_ex) at 1.
-  clear. basic_solver.
-Qed.
-
-Lemma wf_cert_coE : cert_co ≡ ⦗E⦘ ⨾ cert_co ⨾ ⦗E⦘.
-Proof using WF S_in_W ST_in_E IT_new_co.
-  apply wf_new_coE; [apply IST_new_co|apply (wf_coE WF)].
-Qed.
-
-Lemma wf_cert_coD : cert_co ≡ ⦗W⦘ ⨾ cert_co ⨾ ⦗W⦘.
-Proof using WF S_in_W ST_in_E IT_new_co.
-  apply wf_new_coD; [apply IST_new_co|apply (wf_coD WF)].
-Qed.
-
-Lemma wf_cert_col : cert_co ⊆ Gsame_loc.
-Proof using WF S_in_W ST_in_E IT_new_co.
-  apply wf_new_col; [apply IST_new_co|apply (wf_coD WF)].
-Qed.
-
-Lemma cert_co_trans : transitive cert_co.
-Proof using WF S_in_W ST_in_E IT_new_co.
-  apply new_co_trans; try apply WF; apply IST_new_co.
-Qed.
-
-Lemma wf_cert_co_total : forall ol, is_total (E ∩₁ W ∩₁ (fun x => Gloc x = ol)) cert_co.
-Proof using WF S_in_W ST_in_E IT_new_co.
-  intros.
-  apply wf_new_co_total.
-  apply IST_new_co.
-  all: apply WF.
-Qed.
-
-Lemma cert_co_irr : irreflexive cert_co.
-Proof using WF S_in_W ST_in_E IT_new_co.
-  apply new_co_irr. 
-  apply IST_new_co.
-  all: apply WF.
-Qed.
-
-Lemma cert_co_I : cert_co ⨾ ⦗ cert_co_base ⦘ ⊆ Gco ⨾ ⦗ cert_co_base ⦘.
-Proof using WF S_in_W ST_in_E IT_new_co.
-  apply new_co_I.
-  apply IST_new_co.
-  all: apply WF.
-Qed.
-
-Lemma I_co_in_cert_co : ⦗ cert_co_base ⦘ ⨾ Gco ⊆ cert_co.
-Proof using WF S_in_W ST_in_E IT_new_co.
-  apply I_co_in_new_co.
-  apply IST_new_co.
-  all: apply WF.
-Qed.
-
-Lemma cert_co_for_split_helper : ⦗set_compl cert_co_base⦘ ⨾ (immediate cert_co) ⊆ Gsb.
-Proof using All.
-(* Proof using WF S_in_W ST_in_E IT_new_co. *)
-  unfold cert_co.
-  red; intros x y H.
-  assert (A: (E ∩₁ W ∩₁ Tid_ thread) y).
-  { apply (co_for_split IST_new_co (wf_coE WF) (wf_coD WF)).
-    red. eauto. }
-  unfolder in H; desf.
-  assert (B: (E ∩₁ W) x).
-  { hahn_rewrite (wf_new_coE IST_new_co (wf_coE WF)) in H0.
-    hahn_rewrite (wf_new_coD IST_new_co (wf_coD WF)) in H0.
-    unfolder in H0. clear -H0. basic_solver. }
-  apply IST_new_co in B; unfolder in B.
-  destruct B as [B|[[B1 B2] B3]].
-  { intuition. }
-  unfolder in A.
-  assert (D: (⦗ E ∩₁ W ∩₁ Tid_ (tid x) ⦘ ⨾ Gco) x y).
-  { rewrite B3.
-    eapply T_new_co.
-    { apply IST_new_co. }
-    all: try edone; try apply WF.
-    clear -H0 A B1 B2 B3.
-    basic_solver. }
-  desf.
-  eapply same_thread in A0; try edone.
-  { desf.
-    exfalso.
-    unfolder in D; desf.
-    destruct A0.
-    { rewrite H2 in D0. eapply (co_irr WF); edone. }
-    eapply COH.
-    hahn_rewrite <- (@sb_in_hb G).
-    hahn_rewrite <- (@co_in_eco G).
-    clear -H2 D0.
-    basic_solver. }
-  hahn_rewrite (no_co_to_init WF (coherence_sc_per_loc COH)) in D.
-  unfolder in D. apply D.
-Qed.
-
-Lemma cert_co_for_split :
-  ⦗set_compl (GW_ex ∪₁ (I ∪₁ S ∩₁ Tid_ thread))⦘ ⨾ (immediate cert_co) ⊆ Gsb.
-Proof using All.
-  arewrite (immediate cert_co ⊆
-            <|cert_co_base ∪₁ set_compl cert_co_base|> ;; immediate cert_co).
-  { rewrite AuxRel.set_compl_union_id. unfold set_full. by rewrite seq_id_l. }
-  rewrite id_union, seq_union_l, seq_union_r. unionL.
-  2: { rewrite cert_co_for_split_helper. clear. basic_solver. }
-  rewrite <- seqA. rewrite <- id_inter.
-  rewrite set_interC. rewrite <- set_minusE.
-  arewrite (cert_co_base \₁ (GW_ex ∪₁ (I ∪₁ S ∩₁ Tid_ thread)) ⊆₁ ∅).
-  2: clear; basic_solver.
-  unfold cert_co_base. clear. basic_solver.
-Qed.
-
-(* TODO: move to ImmProperties.v *)
-Lemma I_eq_EW_I : I ≡₁ E ∩₁ W ∩₁ I.
-Proof using TCCOH.
-  clear -TCCOH.
-  split; [|clear; basic_solver].
-  generalize (issuedW TCCOH), (issuedE TCCOH).
-  basic_solver.
-Qed.
-
-Lemma cert_co_alt :
-  cert_co  ⊆ Gco ∩ cert_co ⨾ ⦗ cert_co_base ⦘ ∪ ⦗ Tid_ thread ⦘ ⨾ Gco ∩ cert_co ∪ 
-           ⦗ I ∩₁ NTid_ thread ⦘ ⨾ cert_co ⨾ ⦗ (E ∩₁ W ∩₁ Tid_ thread) \₁
-                                              cert_co_base ⦘.
-Proof using All.
-  arewrite (I ∩₁ NTid_ thread ≡₁ cert_co_base \₁ E ∩₁ W ∩₁ Tid_ thread).
-  { rewrite cert_co_base_alt.
-    split.
-    2: { rewrite WF.(W_ex_eq_EW_W_ex), I_eq_EW_I at 1.
-         rewrite set_minus_union_l. unionL.
-         2: { clear. intros x [HH BB]. exfalso. apply BB.
-              generalize HH. basic_solver. }
-         clear. intros x [HH BB]. split; [by apply HH|].
-         generalize HH, BB. basic_solver 10. }
-    clear. intros x [HH BB]. split; [basic_solver|].
-    unfolder. intros AA. desf. }
-  arewrite (cert_co ⊆ cert_co ∩ cert_co) at 1.
-  unfold cert_co at 1.
-  rewrite new_co_in at 1.
-  all: try by apply WF.
-  { clear. basic_solver 40. }
-  apply IST_new_co.
-Qed.
-
-Lemma cert_co_alt' : cert_co  ⊆ Gco ∩ cert_co ∪ 
-  ⦗ I ∩₁ NTid_ thread ⦘ ⨾ cert_co ⨾ ⦗ (E ∩₁ W ∩₁ Tid_ thread) \₁ I ⦘.
-Proof using All.
-  rewrite cert_co_alt at 1.
-  clear.
-  unionL.
-  3: rewrite <- I_in_cert_co_base at 1.
-  all: basic_solver 12.
-Qed.
 
 (******************************************************************************)
 (** Definition of the new rf edges   *)
@@ -2200,9 +2025,6 @@ red; case_refl _.
 - generalize coh_helper; basic_solver 21.
 Qed.
 
-(* TODO: move up *)
-Lemma W_ex_in_cert_co_base : GW_ex ⊆₁ cert_co_base.
-Proof using. unfold cert_co_base. clear. basic_solver. Qed.
 
 Lemma cert_rmw_atomicity : rmw_atomicity certG.
 Proof using WF WF_SC TCCOH AT COH COMP_NTID E_to_S G IT_new_co I_in_S S ST_in_E S_in_W 
@@ -2214,7 +2036,7 @@ Proof using WF WF_SC TCCOH AT COH COMP_NTID E_to_S G IT_new_co I_in_S S ST_in_E 
   red; ins; cut (irreflexive (Cfr ⨾ (cert_co \ Gsb) ⨾ Grmw^{-1})).
   { basic_solver 12. }
   rewrite (rmw_W_ex), !transp_seq, !transp_eqv_rel.
-  unfold cert_co.
+  unfold Cert_co.cert_co.
   rotate 1.
   unfold fr; ins; rewrite transp_union.
   rewrite (dom_rel_helper (dom_rmw_in_D)).
