src/simulation/Cert_co.v
@@ -1,0 +1,300 @@
+From hahn Require Import Hahn.
+
+From imm Require Import Events.
+From imm Require Import Execution.
+From imm Require Import Execution_eco.
+From imm Require Import imm_bob imm_s_ppo.
+From imm Require Import imm_s_hb.
+From imm Require Import imm_s.
+From imm Require Import imm_common_more.
+From imm Require Import CertCOhelper.
+From imm Require Import CombRelations.
+
+Require Import AuxRel2.
+Require Import TraversalConfig.
+Require Import TraversalConfigAlt.
+Require Import TraversalConfigAltOld.
+Require Import ExtTraversalConfig.
+
+Require Import ImmProperties.
+
+Set Implicit Arguments.
+Remove Hints plus_n_O.
+
+Notation "'Tid_' t" := (fun x => tid x = t) (at level 1).
+Notation "'NTid_' t" := (fun x => tid x <> t) (at level 1).
+
+Section CertExec_CO.
+
+Variable G : execution.
+Variable sc : relation actid.
+
+Notation "'Init'" := (fun a => is_true (is_init a)).
+
+Notation "'E'" := G.(acts_set).
+Notation "'Gacts'" := G.(acts).
+Notation "'Glab'" := G.(lab).
+Notation "'Gsb'" := G.(sb).
+Notation "'Grf'" := G.(rf).
+Notation "'Gco'" := G.(co).
+Notation "'Grmw'" := G.(rmw).
+Notation "'Gdata'" := G.(data).
+Notation "'Gaddr'" := G.(addr).
+Notation "'Gctrl'" := G.(ctrl).
+Notation "'Gdeps'" := G.(deps).
+Notation "'Grmw_dep'" := G.(rmw_dep).
+
+Notation "'Gfre'" := G.(fre).
+Notation "'Grfe'" := G.(rfe).
+Notation "'Gcoe'" := G.(coe).
+Notation "'Grfi'" := G.(rfi).
+Notation "'Gfri'" := G.(fri).
+Notation "'Gcoi'" := G.(coi).
+Notation "'Gfr'" := G.(fr).
+Notation "'Geco'" := G.(eco).
+Notation "'Gdetour'" := G.(detour).
+Notation "'Gsw'" := G.(sw).
+Notation "'Grelease'" := G.(release).
+Notation "'Grs'" := G.(rs).
+Notation "'Ghb'" := G.(hb).
+Notation "'Gppo'" := G.(ppo).
+Notation "'Grppo'" := G.(rppo).
+Notation "'Gbob'" := G.(bob).
+Notation "'Gfwbob'" := G.(fwbob).
+Notation "'Gar'" := (G.(ar) sc).
+Notation "'Gar_int'" := (G.(ar_int)).
+Notation "'Gurr'" := (G.(urr) sc).
+Notation "'Gfurr'" := (G.(furr) sc).
+Notation "'Gmsg_rel'" := (G.(msg_rel) sc).
+
+Notation "'Gloc'" := (loc Glab).
+Notation "'Gval'" := (val Glab).
+Notation "'Gsame_loc'" := (same_loc Glab).
+
+Notation "'R'" := (fun a => is_true (is_r Glab a)).
+Notation "'W'" := (fun a => is_true (is_w Glab a)).
+Notation "'F'" := (fun a => is_true (is_f Glab a)).
+Notation "'GR_ex'" := (fun a => is_true (R_ex Glab a)).
+Notation "'GW_ex'" := G.(W_ex).
+Notation "'GW_ex_acq'" := (GW_ex ∩₁ (fun a => is_true (is_xacq Glab a))).
+
+Notation "'Loc_' l" := (fun x => Gloc x = Some l) (at level 1).
+Notation "'W_' l" := (W ∩₁ Loc_ l) (at level 1).
+Notation "'R_' l" := (R ∩₁ Loc_ l) (at level 1).
+
+Notation "'Pln'" := (fun a => is_true (is_only_pln Glab a)).
+Notation "'Rlx'" := (fun a => is_true (is_rlx Glab a)).
+Notation "'Rel'" := (fun a => is_true (is_rel Glab a)).
+Notation "'Acq'" := (fun a => is_true (is_acq Glab a)).
+Notation "'Acqrel'" := (fun a => is_true (is_acqrel Glab a)).
+Notation "'Acq/Rel'" := (fun a => is_true (is_ra Glab a)).
+Notation "'Sc'" := (fun a => is_true (is_sc Glab a)).
+Notation "'xacq'" := (fun a => is_true (is_xacq Glab a)).
+
+Variable T : trav_config.
+Variable S : actid -> Prop.
+
+Notation "'I'" := (issued T).
+Notation "'C'" := (covered T).
+
+Variable thread : BinNums.positive.
+
+Hypothesis WF : Wf G.
+Hypothesis WF_SC : wf_sc G sc.
+Hypothesis RELCOV : W ∩₁ Rel ∩₁ I ⊆₁ C.
+Hypothesis TCCOH : tc_coherent G sc T.
+Hypothesis ACYC_EXT : acyc_ext G sc.
+Hypothesis CSC : coh_sc G sc.
+Hypothesis COH : coherence G.
+Hypothesis AT : rmw_atomicity G.
+
+Hypothesis IT_new_co: I ∪₁ E ∩₁ W ∩₁ Tid_ thread ≡₁ E ∩₁ W.
+Hypothesis S_in_W : S ⊆₁ W.
+Hypothesis ST_in_E : S ∩₁ Tid_ thread ⊆₁ E.
+Hypothesis I_in_S : I ⊆₁ S.
+Hypothesis S_I_in_W_ex : (S ∩₁ Tid_ thread) \₁ I ⊆₁ W_ex G.
+
+Definition cert_co_base := I ∪₁ W_ex G.
+Lemma cert_co_base_alt : cert_co_base ≡₁ I ∪₁ W_ex G ∩₁ Tid_ thread.
+Proof using WF IT_new_co.
+  clear -WF IT_new_co.
+  unfold cert_co_base.
+  split; [|basic_solver].
+  unionL; [basic_solver|].
+  rewrite WF.(W_ex_eq_EW_W_ex) at 1.
+  rewrite <- IT_new_co. basic_solver.
+Qed.
+
+Lemma I_in_cert_co_base : I ⊆₁ cert_co_base.
+Proof using. unfold cert_co_base. basic_solver. Qed.
+
+Lemma IST_in_cert_co_base : I ∪₁ S ∩₁ Tid_ thread ⊆₁ cert_co_base.
+Proof using S_I_in_W_ex.
+  rewrite AuxRel.set_subset_union_minus with (s:=S ∩₁ Tid_ thread) (s':=I).
+  rewrite S_I_in_W_ex.
+  unfold cert_co_base. clear. basic_solver.
+Qed.
+
+Lemma W_ex_in_cert_co_base : GW_ex ⊆₁ cert_co_base.
+Proof using. unfold cert_co_base. clear. basic_solver. Qed.
+
+Definition cert_co := new_co G cert_co_base (E ∩₁ W ∩₁ Tid_ thread).
+
+Lemma IST_new_co : cert_co_base ∪₁ E ∩₁ W ∩₁ Tid_ thread ≡₁ E ∩₁ W.
+Proof using WF S_in_W ST_in_E IT_new_co.
+  rewrite <- IT_new_co at 2.
+  rewrite cert_co_base_alt.
+  rewrite WF.(W_ex_eq_EW_W_ex) at 1.
+  clear. basic_solver.
+Qed.
+
+Lemma wf_cert_coE : cert_co ≡ ⦗E⦘ ⨾ cert_co ⨾ ⦗E⦘.
+Proof using WF S_in_W ST_in_E IT_new_co.
+  apply wf_new_coE; [apply IST_new_co|apply (wf_coE WF)].
+Qed.
+
+Lemma wf_cert_coD : cert_co ≡ ⦗W⦘ ⨾ cert_co ⨾ ⦗W⦘.
+Proof using WF S_in_W ST_in_E IT_new_co.
+  apply wf_new_coD; [apply IST_new_co|apply (wf_coD WF)].
+Qed.
+
+Lemma wf_cert_col : cert_co ⊆ Gsame_loc.
+Proof using WF S_in_W ST_in_E IT_new_co.
+  apply wf_new_col; [apply IST_new_co|apply (wf_coD WF)].
+Qed.
+
+Lemma cert_co_trans : transitive cert_co.
+Proof using WF S_in_W ST_in_E IT_new_co.
+  apply new_co_trans; try apply WF; apply IST_new_co.
+Qed.
+
+Lemma wf_cert_co_total : forall ol, is_total (E ∩₁ W ∩₁ (fun x => Gloc x = ol)) cert_co.
+Proof using WF S_in_W ST_in_E IT_new_co.
+  intros.
+  apply wf_new_co_total.
+  apply IST_new_co.
+  all: apply WF.
+Qed.
+
+Lemma cert_co_irr : irreflexive cert_co.
+Proof using WF S_in_W ST_in_E IT_new_co.
+  apply new_co_irr. 
+  apply IST_new_co.
+  all: apply WF.
+Qed.
+
+Lemma cert_co_I : cert_co ⨾ ⦗ cert_co_base ⦘ ⊆ Gco ⨾ ⦗ cert_co_base ⦘.
+Proof using WF S_in_W ST_in_E IT_new_co.
+  apply new_co_I.
+  apply IST_new_co.
+  all: apply WF.
+Qed.
+
+Lemma I_co_in_cert_co : ⦗ cert_co_base ⦘ ⨾ Gco ⊆ cert_co.
+Proof using WF S_in_W ST_in_E IT_new_co.
+  apply I_co_in_new_co.
+  apply IST_new_co.
+  all: apply WF.
+Qed.
+
+Lemma cert_co_for_split_helper : ⦗set_compl cert_co_base⦘ ⨾ (immediate cert_co) ⊆ Gsb.
+Proof using All.
+(* Proof using WF S_in_W ST_in_E IT_new_co. *)
+  unfold cert_co.
+  red; intros x y H.
+  assert (A: (E ∩₁ W ∩₁ Tid_ thread) y).
+  { apply (co_for_split IST_new_co (wf_coE WF) (wf_coD WF)).
+    red. eauto. }
+  unfolder in H; desf.
+  assert (B: (E ∩₁ W) x).
+  { hahn_rewrite (wf_new_coE IST_new_co (wf_coE WF)) in H0.
+    hahn_rewrite (wf_new_coD IST_new_co (wf_coD WF)) in H0.
+    unfolder in H0. clear -H0. basic_solver. }
+  apply IST_new_co in B; unfolder in B.
+  destruct B as [B|[[B1 B2] B3]].
+  { intuition. }
+  unfolder in A.
+  assert (D: (⦗ E ∩₁ W ∩₁ Tid_ (tid x) ⦘ ⨾ Gco) x y).
+  { rewrite B3.
+    eapply T_new_co.
+    { apply IST_new_co. }
+    all: try edone; try apply WF.
+    clear -H0 A B1 B2 B3.
+    basic_solver. }
+  desf.
+  eapply same_thread in A0; try edone.
+  { desf.
+    exfalso.
+    unfolder in D; desf.
+    destruct A0.
+    { rewrite H2 in D0. eapply (co_irr WF); edone. }
+    eapply COH.
+    hahn_rewrite <- (@sb_in_hb G).
+    hahn_rewrite <- (@co_in_eco G).
+    clear -H2 D0.
+    basic_solver. }
+  hahn_rewrite (no_co_to_init WF (coherence_sc_per_loc COH)) in D.
+  unfolder in D. apply D.
+Qed.
+
+Lemma cert_co_for_split :
+  ⦗set_compl (GW_ex ∪₁ (I ∪₁ S ∩₁ Tid_ thread))⦘ ⨾ (immediate cert_co) ⊆ Gsb.
+Proof using All.
+  arewrite (immediate cert_co ⊆
+            <|cert_co_base ∪₁ set_compl cert_co_base|> ;; immediate cert_co).
+  { rewrite AuxRel.set_compl_union_id. unfold set_full. by rewrite seq_id_l. }
+  rewrite id_union, seq_union_l, seq_union_r. unionL.
+  2: { rewrite cert_co_for_split_helper. clear. basic_solver. }
+  rewrite <- seqA. rewrite <- id_inter.
+  rewrite set_interC. rewrite <- set_minusE.
+  arewrite (cert_co_base \₁ (GW_ex ∪₁ (I ∪₁ S ∩₁ Tid_ thread)) ⊆₁ ∅).
+  2: clear; basic_solver.
+  unfold cert_co_base. clear. basic_solver.
+Qed.
+
+(* TODO: move to ImmProperties.v *)
+Lemma I_eq_EW_I : I ≡₁ E ∩₁ W ∩₁ I.
+Proof using TCCOH.
+  clear -TCCOH.
+  split; [|clear; basic_solver].
+  generalize (issuedW TCCOH), (issuedE TCCOH).
+  basic_solver.
+Qed.
+
+Lemma cert_co_alt :
+  cert_co  ⊆ Gco ∩ cert_co ⨾ ⦗ cert_co_base ⦘ ∪ ⦗ Tid_ thread ⦘ ⨾ Gco ∩ cert_co ∪ 
+           ⦗ I ∩₁ NTid_ thread ⦘ ⨾ cert_co ⨾ ⦗ (E ∩₁ W ∩₁ Tid_ thread) \₁
+                                              cert_co_base ⦘.
+Proof using All.
+  arewrite (I ∩₁ NTid_ thread ≡₁ cert_co_base \₁ E ∩₁ W ∩₁ Tid_ thread).
+  { rewrite cert_co_base_alt.
+    split.
+    2: { rewrite WF.(W_ex_eq_EW_W_ex), I_eq_EW_I at 1.
+         rewrite set_minus_union_l. unionL.
+         2: { clear. intros x [HH BB]. exfalso. apply BB.
+              generalize HH. basic_solver. }
+         clear. intros x [HH BB]. split; [by apply HH|].
+         generalize HH, BB. basic_solver 10. }
+    clear. intros x [HH BB]. split; [basic_solver|].
+    unfolder. intros AA. desf. }
+  arewrite (cert_co ⊆ cert_co ∩ cert_co) at 1.
+  unfold cert_co at 1.
+  rewrite new_co_in at 1.
+  all: try by apply WF.
+  { clear. basic_solver 40. }
+  apply IST_new_co.
+Qed.
+
+Lemma cert_co_alt' : cert_co  ⊆ Gco ∩ cert_co ∪ 
+  ⦗ I ∩₁ NTid_ thread ⦘ ⨾ cert_co ⨾ ⦗ (E ∩₁ W ∩₁ Tid_ thread) \₁ I ⦘.
+Proof using All.
+  rewrite cert_co_alt at 1.
+  clear.
+  unionL.
+  3: rewrite <- I_in_cert_co_base at 1.
+  all: basic_solver 12.
+Qed.
+
+
+
+End CertExec_CO.
